Prove TreeKEM's assumes

fstar/treekem/code/MLS.TreeKEM.API.fst
@@ -32,34 +32,28 @@ let create #bytes #cb dec_key enc_key =
 val welcome:
   #bytes:Type0 -> {|crypto_bytes bytes|} ->
   #l:nat ->
-  treekem bytes l 0 -> hpke_private_key bytes -> option (bytes & nat) -> leaf_ind:nat ->
+  t:treekem bytes l 0{treekem_invariant t} -> hpke_private_key bytes -> option (bytes & nat) -> leaf_ind:nat{leaf_ind < pow2 l /\ Some? (leaf_at t leaf_ind)} ->
   result (treekem_state bytes leaf_ind)
 let welcome #bytes #cb #l t leaf_decryption_key opt_path_secret_and_inviter_ind leaf_ind =
-  if not (leaf_ind < pow2 l) then
-    error "welcome: leaf_index too big"
-  else (
-    let priv = create_empty_priv leaf_decryption_key in
-    let? priv =
-      match opt_path_secret_and_inviter_ind with
-      | None -> return priv
-      | Some (path_secret, inviter_ind) ->
-        if not (leaf_ind <> inviter_ind) then
-          error "welcome: leaf_index and inviter index are the same"
-        else if not (inviter_ind < pow2 l) then
-          error "welcome: inviter_index too big"
-        else
-          let path_secret_level = compute_least_common_ancestor_level priv inviter_ind in
-          let? (priv, _) = path_apply_path t priv path_secret path_secret_level in
-          return priv
-    in
-    assume(treekem_invariant t);
-    assume(treekem_priv_invariant t priv);
-    return {
-      levels = l;
-      tree = t;
-      priv;
-    }
-  )
+  let priv = create_empty_priv leaf_decryption_key in
+  let? priv =
+    match opt_path_secret_and_inviter_ind with
+    | None -> return priv
+    | Some (path_secret, inviter_ind) ->
+      if not (leaf_ind <> inviter_ind) then
+        error "welcome: leaf_index and inviter index are the same"
+      else if not (inviter_ind < pow2 l) then
+        error "welcome: inviter_index too big"
+      else
+        let path_secret_level = compute_least_common_ancestor_level priv inviter_ind in
+        let? (priv, _) = path_apply_path t priv path_secret path_secret_level in
+        return priv
+  in
+  return {
+    levels = l;
+    tree = t;
+    priv;
+  }
 
 (*** Add ***)
 
@@ -70,8 +64,8 @@ val add:
 let add #bytes #cb #leaf_ind st kp =
   match find_empty_leaf st.tree with
   | Some i -> (
-    assume(treekem_invariant (tree_add st.tree i kp));
-    assume(treekem_priv_invariant (tree_add st.tree i kp) st.priv);
+    treekem_invariant_add st.tree i kp;
+    treekem_priv_invariant_add st.tree st.priv i kp;
     ({ st with
       tree = tree_add st.tree i kp;
     }, (i <: nat))
@@ -80,8 +74,10 @@ let add #bytes #cb #leaf_ind st kp =
     find_empty_leaf_tree_extend st.tree;
     let extended_tree = tree_extend st.tree in
     let i = Some?.v (find_empty_leaf extended_tree) in
-    assume(treekem_invariant (tree_add extended_tree i kp));
-    assume(treekem_priv_invariant (tree_add extended_tree i kp) (path_extend st.priv));
+    treekem_invariant_extend st.tree;
+    treekem_priv_invariant_extend st.tree st.priv;
+    treekem_invariant_add extended_tree i kp;
+    treekem_priv_invariant_add extended_tree (path_extend st.priv) i kp;
     ({ st with
       levels = st.levels+1;
       tree = tree_add extended_tree i kp;
@@ -96,8 +92,8 @@ val update:
   st:treekem_state bytes leaf_ind -> treekem_leaf bytes -> treekem_index st ->
   treekem_state bytes leaf_ind
 let update #bytes #cb #leaf_ind st lp i =
-  assume(treekem_invariant (tree_update st.tree i lp));
-  assume(treekem_priv_invariant (tree_update st.tree i lp) st.priv);
+  treekem_invariant_update st.tree i lp;
+  treekem_priv_invariant_update st.tree st.priv i lp;
   { st with tree = tree_update st.tree i lp; }
 
 (*** Remove ***)
@@ -108,18 +104,22 @@ val remove:
   treekem_state bytes leaf_ind
 let remove #bytes #cb #leaf_ind st i =
   let blanked_tree = (tree_remove st.tree i) in
+  treekem_invariant_remove st.tree i;
+  treekem_priv_invariant_remove st.tree st.priv i;
   if TNode? blanked_tree && is_tree_empty (TNode?.right blanked_tree) then (
-    assume(leaf_ind < pow2 (st.levels-1));
-    assume(treekem_invariant (tree_truncate blanked_tree));
-    assume(treekem_priv_invariant (tree_truncate blanked_tree) (path_truncate st.priv));
-    { st with
-      levels = st.levels-1;
-      tree = tree_truncate blanked_tree;
-      priv = path_truncate st.priv;
-    }
+    if leaf_ind >= pow2 (st.levels-1) then (
+      MLS.TreeCommon.Lemmas.is_tree_empty_leaf_at (TNode?.right blanked_tree) leaf_ind;
+      false_elim ()
+    ) else (
+      treekem_invariant_truncate blanked_tree;
+      treekem_priv_invariant_truncate blanked_tree st.priv;
+      { st with
+        levels = st.levels-1;
+        tree = tree_truncate blanked_tree;
+        priv = path_truncate st.priv;
+      }
+    )
   ) else (
-    assume(treekem_invariant blanked_tree);
-    assume(treekem_priv_invariant blanked_tree st.priv);
     { st with
       tree = blanked_tree;
     }
@@ -129,22 +129,22 @@ let remove #bytes #cb #leaf_ind st i =
 
 val commit:
   #bytes:Type0 -> {|crypto_bytes bytes|} -> #leaf_ind:nat ->
-  st:treekem_state bytes leaf_ind -> #li:treekem_index st{li <> leaf_ind} -> p:pathkem bytes st.levels 0 li{path_filtering_ok st.tree p} -> list nat -> group_context_nt bytes ->
+  st:treekem_state bytes leaf_ind -> #li:treekem_index st{li <> leaf_ind} -> p:pathkem bytes st.levels 0 li{path_filtering_ok st.tree p} -> excluded_leaves:list nat{~(List.Tot.memP leaf_ind excluded_leaves)} -> group_context_nt bytes ->
   result (treekem_state bytes leaf_ind & bytes)
 let commit #bytes #cb #leaf_ind st #li p excluded_leaves group_context =
   let un_added_tree = un_add st.tree excluded_leaves in
-  assume(treekem_invariant un_added_tree);
+  treekem_invariant_un_add st.tree excluded_leaves;
+  treekem_priv_invariant_un_add st.tree st.priv excluded_leaves;
   if not (check_update_path_ciphertexts_lengthes un_added_tree p) then (
     error "TreeKEM.commit: bad UpdatePath ciphertext lengths"
   ) else (
-    assume(treekem_priv_invariant un_added_tree st.priv);
     weaken_path_filtering_ok st.tree p;
     path_filtering_weak_ok_un_add st.tree p excluded_leaves;
     let? (path_secret, least_common_ancestor_level) = get_path_secret un_added_tree st.priv p group_context in
     let new_tree = tree_apply_path st.tree p in
     let? (new_priv, root_secret) = path_apply_path new_tree st.priv path_secret least_common_ancestor_level in
-    assume(treekem_invariant new_tree);
-    assume(treekem_priv_invariant new_tree new_priv);
+    treekem_invariant_apply_path st.tree p;
+    treekem_priv_invariant_apply_path st.tree st.priv p path_secret least_common_ancestor_level;
     return ({ st with
       tree = new_tree;
       priv = new_priv;
@@ -174,7 +174,7 @@ let prepare_create_commit #bytes #cb #leaf_ind st rand =
   let path_secret_0, rand = dest_randomness rand in
   let? (path_secrets, commit_secret) = generate_path_secrets st.tree leaf_sk path_secret_0 leaf_ind in
   let? pre_upd_path = path_secrets_to_pre_pathkem path_secrets in
-  assume(path_filtering_ok st.tree path_secrets);
+  path_filtering_ok_generate_path_secrets st.tree leaf_sk path_secret_0 leaf_ind;
   return ({
     path_secrets;
     commit_secret;
@@ -185,7 +185,7 @@ val finalize_create_commit_entropy_lengths:
   st:treekem_state bytes leaf_ind -> list nat ->
   list nat
 let finalize_create_commit_entropy_lengths #bytes #cb #leaf_ind st added_leaves =
-  assume(treekem_invariant (un_add st.tree added_leaves));
+  treekem_invariant_un_add st.tree added_leaves;
   let path_secrets = generate_forgotten_path_secrets st.tree leaf_ind in
   encrypt_path_secrets_entropy_lengths (un_add st.tree added_leaves) path_secrets
 
@@ -204,13 +204,13 @@ val finalize_create_commit:
   randomness bytes (finalize_create_commit_entropy_lengths st added_leaves) ->
   result (create_commit_result st)
 let finalize_create_commit #bytes #cb #leaf_ind #st pending added_leaves group_context randomness =
-  assume(treekem_invariant (un_add st.tree added_leaves));
+  treekem_invariant_un_add st.tree added_leaves;
   let? (update_path, new_priv) = encrypt_path_secrets (un_add st.tree added_leaves) pending.path_secrets group_context randomness in
   let? added_leaves_path_secrets = get_path_secret_of_added_leaves pending.path_secrets added_leaves in
   let new_tree = tree_apply_path st.tree update_path in
-  assume(path_filtering_ok st.tree update_path);
-  assume(treekem_invariant new_tree);
-  assume(treekem_priv_invariant new_tree new_priv);
+  path_filtering_ok_encrypt_path_secrets st.tree (un_add st.tree added_leaves) pending.path_secrets group_context randomness;
+  treekem_invariant_apply_path st.tree update_path;
+  treekem_priv_invariant_encrypt_path_secrets st.tree (un_add st.tree added_leaves) pending.path_secrets group_context randomness;
   return ({
     new_state = { st with
       tree = new_tree;
