fstar/treekem/proofs/MLS.TreeKEM.Invariants.Proofs.fst
@@ -4,10 +4,14 @@ open Comparse
 open MLS.Crypto
 open MLS.Tree
 open MLS.TreeCommon
+open MLS.NetworkTypes
 open MLS.TreeKEM.Operations
 open MLS.TreeKEM.Types
 open MLS.TreeKEM.Invariants
 open MLS.NetworkBinder.Properties
+open MLS.TreeCommon.Lemmas
+open MLS.MiscLemmas
+open MLS.Result
 
 #set-options "--fuel 1 --ifuel 1"
 
@@ -54,3 +58,392 @@ let rec weaken_path_filtering_ok #bytes #cb #l #i #li t p =
   | PNode _ p_next ->
     let (child, _) = get_child_sibling t li in
     weaken_path_filtering_ok child p_next
+
+(*** Extend invariants ***)
+
+val treekem_invariant_mk_blank_tree:
+  #bytes:Type0 -> {|crypto_bytes bytes|} ->
+  l:nat -> i:tree_index l ->
+  Lemma (treekem_invariant #bytes (mk_blank_tree l i))
+let rec treekem_invariant_mk_blank_tree #bytes #cb l i =
+  if l = 0 then ()
+  else (
+    treekem_invariant_mk_blank_tree #bytes (l-1) (left_index i);
+    treekem_invariant_mk_blank_tree #bytes (l-1) (right_index i)
+  )
+
+val treekem_invariant_extend:
+  #bytes:Type0 -> {|crypto_bytes bytes|} ->
+  #l:nat ->
+  t:treekem bytes l 0 ->
+  Lemma
+  (requires treekem_invariant t)
+  (ensures treekem_invariant (tree_extend t))
+let treekem_invariant_extend #bytes #cb #l t =
+  treekem_invariant_mk_blank_tree #bytes l (right_index #(l+1) 0)
+
+val treekem_priv_invariant_extend:
+  #bytes:Type0 -> {|crypto_bytes bytes|} ->
+  #l:nat -> #li:leaf_index l 0 ->
+  t:treekem bytes l 0 -> p:treekem_priv bytes l 0 li ->
+  Lemma
+  (requires treekem_priv_invariant t p)
+  (ensures treekem_priv_invariant (tree_extend t) (path_extend p))
+let treekem_priv_invariant_extend #bytes #cb #l #li t p = ()
+
+(*** Truncate invariants ***)
+
+val treekem_invariant_truncate:
+  #bytes:Type0 -> {|crypto_bytes bytes|} ->
+  #l:pos ->
+  t:treekem bytes l 0{is_tree_empty (TNode?.right t)} ->
+  Lemma
+  (requires treekem_invariant t)
+  (ensures treekem_invariant (tree_truncate t))
+let treekem_invariant_truncate #bytes #cb #l t = ()
+
+val treekem_priv_invariant_truncate:
+  #bytes:Type0 -> {|crypto_bytes bytes|} ->
+  #l:pos -> #li:leaf_index (l-1) 0 ->
+  t:treekem bytes l 0{is_tree_empty (TNode?.right t)} -> p:treekem_priv bytes l 0 li ->
+  Lemma
+  (requires treekem_priv_invariant t p)
+  (ensures treekem_priv_invariant (tree_truncate t) (path_truncate p))
+let treekem_priv_invariant_truncate #bytes #cb #l #li t p = ()
+
+(*** Add invariants ***)
+
+val leaf_at_tree_add:
+  #bytes:Type0 -> {|crypto_bytes bytes|} ->
+  #l:nat -> #i:tree_index l ->
+  t:treekem bytes l i -> li:leaf_index l i -> lp:treekem_leaf bytes ->
+  li':leaf_index l i ->
+  Lemma
+  (leaf_at (tree_add t li lp) li' == (if li = li' then Some lp else leaf_at t li'))
+let rec leaf_at_tree_add #bytes #cb #l #i t li lp li' =
+  match t with
+  | TLeaf _ -> ()
+  | TNode _ left right -> (
+    match is_left_leaf li, is_left_leaf li' with
+    | true, true -> leaf_at_tree_add left li lp li'
+    | false, false -> leaf_at_tree_add right li lp li'
+    | _, _ -> ()
+  )
+
+val treekem_invariant_add:
+  #bytes:Type0 -> {|crypto_bytes bytes|} ->
+  #l:nat -> #i:tree_index l ->
+  t:treekem bytes l i -> li:leaf_index l i -> lp:treekem_leaf bytes ->
+  Lemma
+  (requires treekem_invariant t)
+  (ensures treekem_invariant (tree_add t li lp))
+let rec treekem_invariant_add #bytes #cb #l #i t li lp =
+  match t with
+  | TLeaf _ -> ()
+  | TNode opn _ _ -> (
+    let (child, _) = get_child_sibling t li in
+    treekem_invariant_add child li lp;
+    match opn with
+    | None -> ()
+    | Some pn -> (
+      Comparse.for_allP_eq (unmerged_leaf_exists t) pn.unmerged_leaves;
+      Comparse.for_allP_eq (unmerged_leaf_exists (tree_add t li lp)) (insert_sorted li pn.unmerged_leaves);
+      FStar.Classical.forall_intro (mem_insert_sorted li pn.unmerged_leaves);
+      FStar.Classical.forall_intro (leaf_at_tree_add t li lp)
+    )
+  )
+
+val treekem_priv_invariant_add:
+  #bytes:Type0 -> {|crypto_bytes bytes|} ->
+  #l:nat -> #i:tree_index l -> #my_li:leaf_index l i ->
+  t:treekem bytes l i -> p:treekem_priv bytes l i my_li -> li:leaf_index l i -> lp:treekem_leaf bytes ->
+  Lemma
+  (requires treekem_priv_invariant t p)
+  (ensures treekem_priv_invariant (tree_add t li lp) p)
+let treekem_priv_invariant_add #bytes #cb #l #i #my_li t p li lp =
+  leaf_at_tree_add t li lp my_li
+
+(*** Common Update/Remove invariants ***)
+
+val treekem_invariant_change_path:
+  #bytes:Type0 -> {|crypto_bytes bytes|} ->
+  #l:nat -> #i:tree_index l ->
+  t:treekem bytes l i -> li:leaf_index l i -> content:option (treekem_leaf bytes) ->
+  Lemma
+  (requires treekem_invariant t)
+  (ensures treekem_invariant (tree_change_path t li content None))
+let rec treekem_invariant_change_path #bytes #cb #l #i t li content =
+  match t with
+  | TLeaf _ -> ()
+  | TNode _ _ _ ->
+    let (child, _) = get_child_sibling t li in
+    treekem_invariant_change_path child li content
+
+val treekem_priv_invariant_change_path:
+  #bytes:Type0 -> {|crypto_bytes bytes|} ->
+  #l:nat -> #i:tree_index l -> #my_li:leaf_index l i ->
+  t:treekem bytes l i -> p:treekem_priv bytes l i my_li -> li:leaf_index l i -> content:option (treekem_leaf bytes) ->
+  Lemma
+  (requires
+    (li == my_li ==> Some? content) /\
+    treekem_priv_invariant t p
+  )
+  (ensures treekem_priv_invariant (tree_change_path t li content None) p)
+let rec treekem_priv_invariant_change_path #bytes #cb #l #i #my_li t p li content =
+  match t, p with
+  | TLeaf _, PLeaf _ -> ()
+  | TNode _ _ _, PNode _ p_next -> (
+    if is_left_leaf li = is_left_leaf my_li then (
+      let (child, _) = get_child_sibling t li in
+      treekem_priv_invariant_change_path child (p_next <: treekem_priv bytes (l-1) _ my_li) li content
+    ) else ()
+  )
+
+(*** Update invariants ***)
+
+val treekem_invariant_update:
+  #bytes:Type0 -> {|crypto_bytes bytes|} ->
+  #l:nat -> #i:tree_index l ->
+  t:treekem bytes l i -> li:leaf_index l i -> lp:treekem_leaf bytes ->
+  Lemma
+  (requires treekem_invariant t)
+  (ensures treekem_invariant (tree_update t li lp))
+let treekem_invariant_update #bytes #cb #l #i t li lp =
+  treekem_invariant_change_path t li (Some lp)
+
+val treekem_priv_invariant_update:
+  #bytes:Type0 -> {|crypto_bytes bytes|} ->
+  #l:nat -> #i:tree_index l -> #my_li:leaf_index l i ->
+  t:treekem bytes l i -> p:treekem_priv bytes l i my_li -> li:leaf_index l i -> lp:treekem_leaf bytes ->
+  Lemma
+  (requires treekem_priv_invariant t p)
+  (ensures treekem_priv_invariant (tree_update t li lp) p)
+let treekem_priv_invariant_update #bytes #cb #l #i #my_li t p li lp =
+  treekem_priv_invariant_change_path t p li (Some lp)
+
+(*** Remove invariants ***)
+
+val treekem_invariant_remove:
+  #bytes:Type0 -> {|crypto_bytes bytes|} ->
+  #l:nat -> #i:tree_index l ->
+  t:treekem bytes l i -> li:leaf_index l i ->
+  Lemma
+  (requires treekem_invariant t)
+  (ensures treekem_invariant (tree_remove t li))
+let treekem_invariant_remove #bytes #cb #l #i t li =
+  treekem_invariant_change_path t li None
+
+val treekem_priv_invariant_remove:
+  #bytes:Type0 -> {|crypto_bytes bytes|} ->
+  #l:nat -> #i:tree_index l -> #my_li:leaf_index l i ->
+  t:treekem bytes l i -> p:treekem_priv bytes l i my_li -> li:leaf_index l i ->
+  Lemma
+  (requires
+    my_li <> li /\
+    treekem_priv_invariant t p
+  )
+  (ensures treekem_priv_invariant (tree_remove t li) p)
+let treekem_priv_invariant_remove #bytes #cb #l #i #my_li t p li =
+  treekem_priv_invariant_change_path t p li None
+
+(*** Un-add invariants ***)
+
+val unmerged_leaf_exists_un_add:
+  #bytes:Type0 -> {|crypto_bytes bytes|} ->
+  #l:nat -> #i:tree_index l ->
+  t:treekem bytes l i -> excluded_leaves:list nat ->
+  x:nat ->
+  Lemma
+  (requires
+    unmerged_leaf_exists t x /\
+    ~(List.Tot.mem x excluded_leaves)
+  )
+  (ensures unmerged_leaf_exists (un_add t excluded_leaves) x)
+let rec unmerged_leaf_exists_un_add #bytes #cb #l #i t excluded_leaves x =
+  match t with
+  | TLeaf _ -> ()
+  | TNode _ left right -> (
+    let x: leaf_index l i = x in
+    if is_left_leaf x then (
+      unmerged_leaf_exists_un_add left excluded_leaves x
+    ) else (
+      unmerged_leaf_exists_un_add right excluded_leaves x
+    )
+  )
+
+val treekem_invariant_un_add:
+  #bytes:Type0 -> {|crypto_bytes bytes|} ->
+  #l:nat -> #i:tree_index l ->
+  t:treekem bytes l i -> excluded_leaves:list nat ->
+  Lemma
+  (requires treekem_invariant t)
+  (ensures treekem_invariant (un_add t excluded_leaves))
+let rec treekem_invariant_un_add #bytes #cb #l #i t excluded_leaves =
+  match t with
+  | TLeaf _ -> ()
+  | TNode opn left right -> (
+    treekem_invariant_un_add left excluded_leaves;
+    treekem_invariant_un_add right excluded_leaves;
+    match opn with
+    | None -> ()
+    | Some pn -> (
+      Comparse.for_allP_eq (unmerged_leaf_exists t) pn.unmerged_leaves;
+      Comparse.for_allP_eq (unmerged_leaf_exists (un_add t excluded_leaves)) (List.Tot.filter (excluded_pre excluded_leaves) pn.unmerged_leaves);
+      FStar.Classical.forall_intro (mem_filter (excluded_pre excluded_leaves) pn.unmerged_leaves);
+      FStar.Classical.forall_intro (FStar.Classical.move_requires (unmerged_leaf_exists_un_add t excluded_leaves))
+    )
+  )
+
+val leaf_at_un_add:
+  #bytes:Type0 -> {|crypto_bytes bytes|} ->
+  #l:nat -> #i:tree_index l ->
+  t:treekem bytes l i -> excluded_leaves:list nat ->
+  li:leaf_index l i ->
+  Lemma (leaf_at (un_add t excluded_leaves) li = (if List.Tot.mem li excluded_leaves then None else leaf_at t li))
+let rec leaf_at_un_add #bytes #cb #l #i t excluded_leaves li =
+  match t with
+  | TLeaf _ -> ()
+  | TNode _ _ _ ->
+    let (child, _) = get_child_sibling t li in
+    leaf_at_un_add child excluded_leaves li
+
+val treekem_priv_invariant_un_add:
+  #bytes:Type0 -> {|crypto_bytes bytes|} ->
+  #l:nat -> #i:tree_index l -> #li:leaf_index l i ->
+  t:treekem bytes l i -> p:treekem_priv bytes l i li -> excluded_leaves:list nat ->
+  Lemma
+  (requires
+    ~(List.Tot.memP li excluded_leaves) /\
+    treekem_priv_invariant t p
+  )
+  (ensures treekem_priv_invariant (un_add t excluded_leaves) p)
+let treekem_priv_invariant_un_add #bytes #cb #l #i #li t p excluded_leaves =
+  leaf_at_un_add t excluded_leaves li
+
+(*** Apply path invariants ***)
+
+val treekem_invariant_apply_path:
+  #bytes:Type0 -> {|crypto_bytes bytes|} ->
+  #l:nat -> #i:tree_index l -> #li:leaf_index l i ->
+  t:treekem bytes l i -> p:pathkem bytes l i li ->
+  Lemma
+  (requires treekem_invariant t)
+  (ensures treekem_invariant (tree_apply_path t p))
+let rec treekem_invariant_apply_path #bytes #cb #l #i #li t p =
+  match t, p with
+  | TLeaf _, PLeaf _ -> ()
+  | TNode _ _ _, PNode _ p_next -> (
+    let (child, _) = get_child_sibling t li in
+    treekem_invariant_apply_path child p_next
+  )
+
+val leaf_at_tree_apply_path:
+  #bytes:Type0 -> {|crypto_bytes bytes|} ->
+  #l:nat -> #i:tree_index l -> #li:leaf_index l i ->
+  t:treekem bytes l i -> p:pathkem bytes l i li ->
+  li':leaf_index l i ->
+  Lemma (leaf_at (tree_apply_path t p) li' = (if li = li' then Some (get_path_leaf p) else leaf_at t li'))
+let rec leaf_at_tree_apply_path #bytes #cb #l #i #li t p li' =
+  match t, p with
+  | TLeaf _, PLeaf _ -> ()
+  | TNode _ left right, PNode _ p_next ->
+    match is_left_leaf li, is_left_leaf li' with
+    | true, true -> leaf_at_tree_apply_path left p_next li'
+    | false, false -> leaf_at_tree_apply_path right p_next li'
+    | _, _ -> ()
+
+val treekem_priv_invariant_apply_path:
+  #bytes:Type0 -> {|crypto_bytes bytes|} ->
+  #l:nat -> #i:tree_index l -> #my_li:leaf_index l i -> #li:leaf_index l i ->
+  t:treekem bytes l i -> priv:treekem_priv bytes l i my_li -> p:pathkem bytes l i li ->
+  path_secret:bytes -> path_node_level:path_secret_level l ->
+  Lemma
+  (requires treekem_priv_invariant t priv)
+  (ensures (
+    match path_apply_path (tree_apply_path t p) priv path_secret path_node_level with
+    | Success (new_path, _) -> treekem_priv_invariant (tree_apply_path t p) new_path
+    | _ -> True
+  ))
+let treekem_priv_invariant_apply_path #bytes #cb #l #i #my_li #li t priv p path_secret path_node_level =
+  leaf_at_tree_apply_path t p my_li
+
+(*** Create commit invariants ***)
+
+val path_filtering_ok_generate_path_secrets:
+  #bytes:Type0 -> {|crypto_bytes bytes|} ->
+  #l:nat -> #i:tree_index l ->
+  t:treekem bytes l i ->
+  leaf_sk:hpke_private_key bytes -> path_secret_0:bytes -> li:leaf_index l i ->
+  Lemma (
+    match generate_path_secrets t leaf_sk path_secret_0 li with
+    | Success (res, _) -> path_filtering_ok t res
+    | _ -> True
+  )
+let rec path_filtering_ok_generate_path_secrets #bytes #cb #l #i t leaf_sk path_secret_0 li =
+  match generate_path_secrets t leaf_sk path_secret_0 li with
+  | Success (res, _) -> (
+    match t with
+    | TLeaf _ -> ()
+    | TNode _ _ _ -> (
+      let (child, sibling) = get_child_sibling t li in
+      path_filtering_ok_generate_path_secrets child leaf_sk path_secret_0 li
+    )
+  )
+  | _ -> ()
+
+#push-options "--z3rlimit 25"
+// ref_t corresponds to the actual tree, which is used to compute filtered nodes
+// t corresponds to the un-added tree, used to perform encryption
+val path_filtering_ok_encrypt_path_secrets:
+  #bytes:Type0 -> {|crypto_bytes bytes|} ->
+  #l:nat -> #i:tree_index l -> #li:leaf_index l i ->
+  ref_t:treekem bytes l i ->
+  t:treekem bytes l i{treekem_invariant t} -> p:path_secrets bytes l i li ->
+  group_context:group_context_nt bytes ->
+  rand:randomness bytes (encrypt_path_secrets_entropy_lengths t (forget_path_secrets p)) ->
+  Lemma
+  (requires path_filtering_ok ref_t p)
+  (ensures (
+    match encrypt_path_secrets t p group_context rand with
+    | Success (res, _) -> path_filtering_ok ref_t res
+    | _ -> True
+  ))
+let rec path_filtering_ok_encrypt_path_secrets #bytes #cb #l #i #li ref_t t p group_context rand =
+  match encrypt_path_secrets t p group_context rand with
+  | Success (res, _) -> (
+    match t, p with
+    | TLeaf _, PLeaf leaf_ikm -> ()
+    | TNode _ _ _, PNode None p_next -> (
+      let (child, _) = get_child_sibling t li in
+      let (ref_child, _) = get_child_sibling ref_t li in
+      path_filtering_ok_encrypt_path_secrets ref_child child p_next group_context rand
+    )
+    | TNode _ _ _, PNode (Some path_secret) p_next -> (
+      let (child, sibling) = get_child_sibling t li in
+      let (ref_child, _) = get_child_sibling ref_t li in
+      let rand_cur, rand_next = split_randomness rand in
+      let _ = multi_encrypt_with_label (tree_resolution sibling) "UpdatePathNode" (serialize _ group_context) path_secret rand_cur in
+      path_filtering_ok_encrypt_path_secrets ref_child child p_next group_context rand_next
+    )
+  )
+  | _ -> ()
+#pop-options
+
+val treekem_priv_invariant_encrypt_path_secrets:
+  #bytes:Type0 -> {|crypto_bytes bytes|} ->
+  #l:nat -> #i:tree_index l -> #li:leaf_index l i ->
+  ref_t:treekem bytes l i ->
+  t:treekem bytes l i{treekem_invariant t} -> p:path_secrets bytes l i li ->
+  group_context:group_context_nt bytes ->
+  rand:randomness bytes (encrypt_path_secrets_entropy_lengths t (forget_path_secrets p)) ->
+  Lemma (
+    match encrypt_path_secrets t p group_context rand with
+    | Success (res, new_priv) -> treekem_priv_invariant (tree_apply_path ref_t res) new_priv
+    | _ -> True
+  )
+let treekem_priv_invariant_encrypt_path_secrets #bytes #cb #l #i #li ref_t t p group_context rand =
+  match encrypt_path_secrets t p group_context rand with
+  | Success (res, new_priv) -> (
+    leaf_at_tree_apply_path ref_t res li
+  )
+  | _ -> ()
